Source/DafnyStandardLibraries/src/Std/Frames.dfy
@@ -28,7 +28,8 @@ module Std.Frames {
 
     twostate predicate ValidChange()
       reads this, Repr
-      ensures ValidChange() ==> old(Valid()) && Valid()
+      ensures ValidChange() ==>
+        old(Valid()) && Valid() && fresh(Repr - old(Repr))
 
     twostate lemma ValidImpliesValidChange()
       requires old(Valid())
